specs/L2InteropHandler/L2InteropHandler/Common/block_9202511772071282510_user.lean
@@ -12,12 +12,13 @@ section
 
 open Clear EVMState Ast Expr Stmt FunctionDefinition State Interpreter ExecLemmas OutOfFuelLemmas Abstraction YulNotation PrimOps ReasoningPrinciple Utilities generated.L2InteropHandler L2InteropHandler
 
-def A_block_9202511772071282510 (s₀ s₉ : State) : Prop := sorry
+def A_block_9202511772071282510 (s₀ s₉ : State) : Prop := block_9202511772071282510_concrete_of_code.1 s₀ s₉
 
 lemma block_9202511772071282510_abs_of_concrete {s₀ s₉ : State} :
   Spec block_9202511772071282510_concrete_of_code s₀ s₉ →
   Spec A_block_9202511772071282510 s₀ s₉ := by
-  sorry
+  intro h
+  simpa [A_block_9202511772071282510] using h
 
 end
 
